Languages, semantics, compilers and theorems
Define languages through behavior relations, then semantics from those.

Functional compilers are defined in addition to the existing, relational
ones. Here, typing information is discarded and the usual metatheorems
can be used to reconnect the varions pairs. Messages in particular are
slightly trickier than the others.

Based on all this, define both the compilation chain and state the
target top-level theorem.

Diff/InstanceMarco.v
@@ -1,8 +1,11 @@
 (* MARCO: personal note: on sublimetext, use sublimecoq-run and the menu-noted *)
 
-(* Require Import TraceModel.
+Require Import TraceModel.
 Require Import LanguageModel.
-Require Import ChainModel. *)
+Require Import ChainModel.
+Require Import NonRobustTraceCriterion.
+
+Set Bullet Behavior "Strict Subproofs".
 
 Module Source.
 
@@ -140,6 +143,15 @@ Module Source.
   Inductive sbeh : ss -> sq -> Prop :=
     | B_Sing : forall ss1 sq1 , sbsem ss1 sq1 Skip -> sbeh ss1 sq1.
 
+  (* source language with vacuous context linking *)
+  Definition slang := Build_Language (fun (par : ss) (_ : unit) => par).
+
+  (* source semantics *)
+  Theorem exists_trace : forall s, exists q, sbeh s q.
+  Admitted.
+
+  Definition ssemt := Build_Semantics slang sbeh exists_trace.
+
 End Source.
 
 Module Target.
@@ -245,6 +257,15 @@ Module Target.
   Inductive tbeh : ts -> tq -> Prop :=
     | B_Sing : forall ts1 tq1 , tbsem ts1 tq1 Skip -> tbeh ts1 tq1.
 
+  (* source language with vacuous context linking *)
+  Definition tlang := Build_Language (fun (par : ts) (_ : unit) => par).
+
+  (* source semantics *)
+  Theorem exists_trace : forall s, exists q, tbeh s q.
+  Admitted.
+
+  Definition tsemt := Build_Semantics tlang tbeh exists_trace.
+
 End Target.
 
 Module Compiler.
@@ -260,6 +281,15 @@ Module Compiler.
     | CMPE_P1 : forall se1 st1 te1, S.swte (S.P1 se1) st1 -> cmpe se1 st1 te1 -> cmpe (S.P1 se1) st1 (T.P1 te1)
     | CMPE_P2 : forall se1 st1 te1, S.swte (S.P2 se1) st1 -> cmpe se1 st1 te1 -> cmpe (S.P2 se1) st1 (T.P2 te1).
 
+  Fixpoint cmpe' (se : S.se) : T.te :=
+    match se with
+    | S.Num n => T.Num n
+    | S.Op se1 se2 => T.Op (cmpe' se1) (cmpe' se2)
+    | S.Pair se1 se2 => T.Pair (cmpe' se1) (cmpe' se2)
+    | S.P1 se1 => T.P1 (cmpe' se1)
+    | S.P2 se2 => T.P2 (cmpe' se2)
+    end.
+
   (*given a source expression with a type, translate that into a target sequence.*)
   Inductive gensend : S.se -> S.st -> T.ts -> Prop :=
     | Snd_Base : forall n1 n2 n1' n2', 
@@ -272,12 +302,30 @@ Module Compiler.
       gensend (S.P2 se1) (st1) (ts2) ->
       gensend (se1) (S.Times st1 st2) (T.Seq ts1 ts2).
 
+  Fixpoint gensend' (se : S.se) : T.ts :=
+    match se with
+    | S.Pair (S.Num n1) (S.Num n2) => T.Seq (T.Send (T.Num n1)) (T.Send (T.Num n2))
+    | S.Pair se1 se2 => T.Seq (gensend' se1) (gensend' se2)
+    | _ => T.Skip (* bad case *)
+    end.
+
   (*compile statements*)
   Inductive cmp : S.ss -> T.ts -> Prop :=
     | CMP_Skip : cmp S.Skip T.Skip
     | CMP_Ifz : forall seg ss1 ss2 teg ts1 ts2, S.swts (S.Ifz seg ss1 ss2)-> cmpe seg S.Nat teg -> cmp ss1 ts1 -> cmp ss2 ts2 -> cmp (S.Ifz seg ss1 ss2) (T.Ifz teg ts1 ts2)
+    (* RB: What information is te1 giving us here? *)
     | CMP_Send : forall se1 st1 te1 ts1, S.swts (S.Send se1) -> cmpe se1 st1 te1 -> gensend se1 st1 ts1 -> cmp (S.Send se1) ts1
     | CMP_Seq : forall ss1 ss2 ts1 ts2, S.swts (S.Seq ss1 ss2) -> cmp ss1 ts1 -> cmp ss2 ts2 -> cmp (S.Seq ss1 ss2) (T.Seq ts1 ts2).
+
+  Fixpoint cmp' (ss : S.ss) : T.ts :=
+    match ss with
+    | S.Skip => T.Skip
+    | S.Ifz seg ss1 ss2 => T.Ifz (cmpe' seg) (cmp' ss1) (cmp' ss2)
+    | S.Send se1 => gensend' se1
+    | S.Seq ss1 ss2 => T.Seq (cmp' ss1) (cmp' ss2)
+    end.
+
+  Definition chain := Build_CompilationChain S.slang T.tlang cmp' cmp' id.
 
 End Compiler.
 
@@ -333,4 +381,7 @@ Module RTC.
   Module C := Compiler.
   Module R := TraceRelation.
 
+  Theorem RTC :
+    rel_TC Compiler.chain Source.ssemt Target.tsemt TraceRelation.trel_q.
+  Admitted.
 End RTC.
